slide_sorted

sort/simplest01.v
@@ -6,34 +6,45 @@ From mathcomp Require Import ssreflect ssrnat ssrbool eqtype.
 Fixpoint slide (i:nat) (l:list nat) :=
   match l with
   | [] => (i, [])
-  | h :: t => if i < h then (fun p => (fst p, i :: snd p)) (slide h t)
-              else (fun p => (fst p, h :: snd p)) (slide i t)
+  | h :: t => 
+    if i < h then 
+      match slide h t with (h', t') => (h', i :: t') end
+    else 
+      match slide i t with (i', t') => (i', h :: t') end
   end.
 
-Lemma slide_hold_length : forall i l, length l = length (snd (slide i l)).
+Lemma snd_destr_comm : forall i (al:nat * list nat), 
+  snd (let (a, l) := al in (a, i :: l)) = i :: snd al.
+Proof. move=> i [a l]; done. Qed.
+
+Lemma slide_hold_length : forall i l, 
+  length l = length (snd (slide i l)).
 Proof.
-  fix slide_hold_length 2.
-  intros i. destruct l as [|a l']. simpl. done. simpl. case_eq (i < a); intros H; simpl; apply f_equal; apply slide_hold_length.
+  fix slide_hold_length 2. move=> i [| a l']; rewrite /=. done.
+  case H : (i < a); rewrite snd_destr_comm /=; apply f_equal, slide_hold_length.
 Qed.
 
-Compute slide 1 [5;3;4;2].
-Compute slide 3 [1;5;4;2].
-
-Program Fixpoint sort' (l1:list nat) (l2:list nat) {measure (length l2)} : (list nat) * (list nat):=
+Program Fixpoint sort' (l1:list nat) (l2:list nat) {measure (length l2)} 
+: (list nat) * (list nat):=
   match l2 with
   | [] => (l1, [])
-  (* | h :: t => (fun p1 => (fun p2 => sort' ((snd p1) ++ [fst p2]) (snd p2)) (slide (fst p1) t)) (slide h l1) *)
-  | h :: t => sort' ((snd (slide h l1)) ++ [fst (slide (fst (slide h l1)) t)]) (snd (slide (fst (slide h l1)) t))
+  | h :: t => match slide h l1 with
+      (i, l1') => match slide i t with
+        (i', l2') => sort' (l1' ++ [i']) l2'
+      end
+    end
   end.
 Obligation 1.
-simpl. pose (slide_hold_length (fst (slide h l1)) t) as e. rewrite -e. done.
+rewrite /=. assert (l2' = snd (slide i t)). by rewrite -Heq_anonymous.
+by rewrite H -slide_hold_length.
 Qed.
 
-Definition sort (l:list nat) :=
-  (fun p => fst p ++ snd p) (sort' [] l).
+Definition sort (l:list nat) := fst (sort' [] l).
 
-Compute sort [3;1;4;1;5;9;2;6;5;3;5].
-Compute sort [1;2;3;4;5;6;7].
+Compute sort [3;1;4;1;5;9;2;6;5;3;5]. 
+Compute slide 5 [1;4;7;9].  
+Goal sort [3;1;4;1;5;9;2;6;5;3;5] = [1; 1; 2; 3; 3; 4; 5; 5; 5; 6; 9].
+Proof. by compute. Qed.
 
 Inductive sorted : list nat -> Prop :=
 | sorted_nil : sorted []
@@ -42,122 +53,99 @@ Inductive sorted : list nat -> Prop :=
     x <= y -> sorted (y :: l) -> sorted (x :: y :: l).
 
 Lemma cons_sorted : forall h t, sorted (h :: t) -> sorted t.
-Proof.
-  intros h t S. inversion S. apply sorted_nil. apply H2.
-Qed.
+Proof. intros h t S; inversion S; [apply sorted_nil | apply H2]. Qed.
 
 Lemma cons_cons_sorted : forall a h t, sorted (a :: h :: t) -> sorted (a :: t).
 Proof.
   intros a h [|h2 t'] S. apply sorted_1. inversion S. inversion H3.
-  apply sorted_cons. apply (leq_trans H1 H6). apply H8.
+  apply (sorted_cons _ _ _ (leq_trans H1 H6) H8).
 Qed.
-(* 
-Lemma uo : forall n l1 a l2, sorted (n :: l1 ++ a :: l2) -> sorted ((n :: l1) ++ l2).
-Proof.
-  intros n. induction l1. intros a l2. simpl. apply cons_cons_sorted.
-  intros b l3. simpl. intros S. inversion S.
-  inversion H3. apply cons_sorted. *)
-(* 
-Lemma append_sorted : forall l1 l2, sorted (l1 ++ l2) -> sorted l1 /\ sorted l2.
-Proof.
-  fix append_sorted 1.
-  destruct l1; simpl. intros l2 S. apply conj. apply sorted_nil. apply S.
-  intros l2 S.  elim S.
-  
-  induction l2; simpl. done. intros S. apply conj.
-  apply sorted_nil. apply S. rewrite app_nil_r. intros S. apply conj.
-  apply S. apply sorted_nil. intros S. apply conj.
-   intros l2 S. apply conj.
 
-  induction l1, l2; simpl; intros S. done.
-  apply conj. apply sorted_nil. apply S.  apply conj.
-  by rewrite app_nil_r in S. apply sorted_nil. apply conj.
-   
-  assert (l1 ++ [] = l1). by rewrite app_nil_r. 
-  apply S.
-  assert (l1 ++ [::])
-  Check ((a :: l1) ++ [::]).  *)
+Lemma leq_lt : forall n m, (n < m) = false -> n <= m -> n = m.
+Proof. 
+  move=> n m. rewrite ltnNge. move/eqP/eqP => Nlt Hle.
+  assert (m <= n) as Hge. { apply Nlt. }
+  move: (conj Hle Hge). move/andP. rewrite -eqn_leq. by move/eqP.
+Qed.
 
-   
+Lemma indep_prod : forall (A B C:Type) (f:A -> B -> C) (ab:A*B),
+  (let (a, b) := ab in (f a b)) = f (fst ab) (snd ab).
+Proof. intuition. Qed.
 
-
-Lemma slide_cons : forall a l, sorted (a :: l) -> a :: l = (snd (slide a l)) ++ [fst (slide a l)].
+Lemma slide_cons : forall a l, 
+  sorted (a :: l) -> a :: l = (let (a', l') := slide a l in (l' ++ [a'])).
 Proof.
   fix slide_cons 2.
-  intros a [|h t] S; simpl. done. case_eq (a < h); intros H; simpl.
-  apply f_equal. inversion S. apply slide_cons, H4.
-  inversion S.  pose (cons_cons_sorted a h t S) as S2.
-  pose (slide_cons _ _ S2) as e. assert (h :: (snd (slide a t)) ++  [(fst (slide a t))] = h :: ((snd (slide a t)) ++ [fst (slide a t)])).
-  apply app_comm_cons. rewrite -e. move: H H2. rewrite ltnNge. 
-  move /eqP/eqP.  fold leq. intros H2 H9. fold leq in H2.
-  assert (h <= a). apply H2. pose (conj H H9). 
-  move: a0. move /andP=> a0. rewrite -eqn_leq in a0. 
-  move:a0. move/eqP=> a0. by case a0.
+  intros a [|h t] S; rewrite /=. done. 
+  rewrite 3!indep_prod. case H: (a < h) => /=.
+   - apply f_equal. inversion S. 
+    by rewrite (slide_cons _ _ H4) indep_prod.
+   - inversion S. case (leq_lt _ _ H H2). apply f_equal.
+    rewrite slide_cons. by rewrite indep_prod. apply (cons_cons_sorted _ _ _ S).
 Qed.
 
-Lemma leq_cons_sorted : forall a h l, sorted (h :: l) -> a <= h -> sorted (a :: h :: l).
-Proof.
-  fix leq_cons_sorted 3.
-  intros a h [|n l'] S. intros H. apply sorted_cons. apply H. apply sorted_1.
-  intros H. apply sorted_cons. apply H. apply S.
-Qed.
+Lemma leq_cons_sorted : forall a h l, 
+  sorted (h :: l) -> a <= h -> sorted (a :: h :: l).
+Proof. move=> a h [|n l'] S H; apply sorted_cons; [apply H|apply sorted_1|apply H|apply S]. Qed.
 
-Lemma leq_all_cons_sorted : forall h a t, sorted (h :: t) -> h <= a -> 
-  sorted (snd (slide a t) ++ [fst (slide a t)]) -> sorted (h :: snd (slide a t) ++ [fst (slide a t)]).
+Lemma leq_all_cons_sorted : forall a i l, 
+  sorted (a :: l) -> a <= i -> 
+  sorted (let (h, t) := slide i l in t ++ [h]) ->
+  sorted (let (h, t) := slide i l in a :: t ++ [h]).
 Proof.
-  fix leq_all_cons_sorted 3.
-  intros h a [|i l']; simpl. intros S Hle.
-  apply sorted_cons. apply Hle.
-  intros S Hle. case_eq (a < i); intros H; simpl; intros S2.
-  apply sorted_cons. apply Hle. apply S2. apply sorted_cons.
-  inversion S. apply H2. apply S2.
+  move=> a i [|h t] S Hle /=.
+   - apply sorted_cons, Hle.
+   - rewrite 4!indep_prod; case H: (i < h) => S2 /=.
+    apply (sorted_cons _ _ _ Hle), S2.
+    inversion S. apply (sorted_cons _ _ _ H2 S2).
 Qed.
 
 Lemma slide_sorted' : forall a l, sorted l -> 
-  sorted ((snd (slide a l)) ++ [fst (slide a l)]).
+  sorted (let (h, t) := slide a l in t ++ [h]).
 Proof.
   fix slide_sorted' 2.
-  intros a [|h t] S; simpl. apply sorted_1. case_eq (a < h); intros H; simpl.
-  pose (cons_sorted _ _ S) as S2.
-  pose (slide_sorted' h _ S2).
-  apply leq_all_cons_sorted. assert (sorted (a :: h :: t)).
-  apply sorted_cons. apply ltnW. apply H. apply S. apply (cons_cons_sorted _ _ _ H0).
-  apply ltnW, H. apply slide_sorted'. apply (cons_sorted _ _ S).
-  apply leq_all_cons_sorted. apply S. move: H. rewrite ltnNge. move/eqP/eqP => H.
-  apply H. apply slide_sorted'. apply (cons_sorted _ _ S).
-Qed.
+  move=> a [|h t] S /=. apply sorted_1. case H: (a < h); rewrite 2!indep_prod /=;
+  rewrite -(indep_prod _ _ _ (fun w1 w2 => _ :: w2 ++ [w1])); apply leq_all_cons_sorted.
+   - apply (cons_cons_sorted _ h _), (leq_cons_sorted _ _ _ S), ltnW, H.  
+   - apply ltnW, H.
+   - apply slide_sorted', (cons_sorted _ _ S).
+   - apply S.
+   - move:H. rewrite ltnNge. by move/eqP/eqP.
+   - apply slide_sorted', (cons_sorted _ _ S).
+Qed. 
 
-
-(* Lemma slide_front : forall h t, sorted (h :: t) -> 
- *)
-
-Lemma app_cons_comm : forall (l1:list nat) n l2, l1 ++ n :: l2 = (l1 ++ [n]) ++ l2.
-Proof.
-  induction l1. intros n l2. done.
-  intros n l2. rewrite -app_comm_cons -app_comm_cons -app_comm_cons. apply f_equal.
-  apply IHl1.
-Qed.
+Lemma app_cons_comm : forall A (l1:list A) n l2, 
+  l1 ++ n :: l2 = (l1 ++ [n]) ++ l2.
+Proof. induction l1; by [|move=>n l2; rewrite -3!app_comm_cons IHl1]. Qed.
 
 Lemma sorted_snoc : forall l n, sorted (l ++ [n]) -> sorted l.
 Proof.
   induction l; intros n S. apply sorted_nil. rewrite -app_comm_cons in S.
-  induction l. apply sorted_1. apply sorted_cons. inversion S. apply H1.
-  inversion S. apply cons_sorted in S. apply (IHl _ S).
+  induction l. apply sorted_1. inversion S. apply sorted_cons. apply H1.
+  apply cons_sorted in S. apply (IHl _ S).
 Qed.
-
 
 Lemma app_sorted : forall l1 l2, sorted (l1 ++ l2) -> sorted l1.
 Proof.
   fix app_sorted 2.
-  intros l1. destruct l2.
-  rewrite app_nil_r. apply.
-  rewrite app_cons_comm. intros S. pose (app_sorted _ _ S) as S2.
+  move => l1 [|n l2].
+  (* intros l1. destruct l2. *)
+  by rewrite app_nil_r.
+  rewrite app_cons_comm => S. pose (app_sorted _ _ S) as S2.
   by apply sorted_snoc in S2.
 Qed.
 
+Lemma slide_sorted : forall a l, sorted l -> sorted (snd (slide a l)).
+Proof. 
+  intros a l S. pose (slide_sorted' a _ S) as S2. move:S2.
+  rewrite indep_prod. apply app_sorted.
+Qed.
 
-Lemma insert_sorted : forall a l, sorted l -> sorted (snd (slide a l)).
-Proof. intros a l S; apply (app_sorted _ _ (slide_sorted' _ _ S)). Qed.
-
-
+(* Lemma sort'_sorted : forall l1 l2, sorted l1 -> sorted (fst (sort' l1 l2)).
+Proof.
+  fix sort'_sorted 2.
+  intros l1. destruct l2. intros S.  simpl. apply S.
+  intros S. 
+  unfold sort', sort'_func. apply slide_sorted. simpl. snd. simpl. 
+  Print sort'_func. *)
 
